src/program_proof/fencing/client_proof.v
@@ -1,0 +1,34 @@
+From Perennial.program_proof Require Import grove_prelude.
+From Goose.github_com.mit_pdos.gokv.fencing Require Import client.
+From Perennial.program_proof Require Import grove_prelude.
+From Perennial.program_proof.grove_shared Require Export erpc_lib urpc_proof urpc_spec.
+From Perennial.program_proof.fencing Require Export config_proof frontend_proof.
+From Perennial.program_proof Require Export marshal_proof.
+From iris.base_logic Require Import mono_nat.
+From Perennial.goose_lang Require Import prelude ffi.grove_exit_axiom.
+
+Module client.
+Section client_proof.
+Context `{!heapGS Σ}.
+
+Record client_names :=
+  {
+    config_gn: config.names;
+  }.
+
+Implicit Type γ : client_names.
+Context `{!urpcregG Σ}.
+
+(* This is "own" not "is" because the frontendCk field is written to inside of
+   FetchAndIncrement, so it's actually not safe for one Clerk to have concurrent
+   FAIs. *)
+Definition own_Clerk γ ck : iProp Σ :=
+  ∃ (configCk frontendCk:loc),
+  "HconfigCk" ∷ ck ↦[client.Clerk :: "configCk"] #configCk ∗
+  "HfrontendCk" ∷ ck ↦[client.Clerk :: "frontendCk"] #frontendCk ∗
+
+  "HconfigCk_own" ∷ config.is_Clerk γ.(config_gn) configCk (λ _, True) (λ _, True)
+.
+
+End client_proof.
+End client.
